first self-consistent spec (& proofs of validPageDb) for dynamic allocation
SMCs to allocate and remove "spare" pages, which can also happen during runtime

SVCs to map spare pages as either secure data pages or L2 page tables

verified/pagedb.s.dfy
@@ -181,9 +181,7 @@ predicate validPageDbEntryTyped(d: PageDb, n: PageNr)
        || (entry.L2PTable? && validL2PTable(d, n))
        || (entry.Dispatcher? && (entry.entered ==>
             validDispatcherContext(entry.ctxt)))
-       // AFAIK the only requirements we need to specify about data pages are 
-       // covered by wellFormedPageDbTyped
-       || (entry.DataPage?))
+       || entry.DataPage? || entry.SparePage?)
 }
 
 predicate isAddrspace(d: PageDb, n: int)
@@ -309,6 +307,11 @@ function initialPageDb(): PageDb
 //-----------------------------------------------------------------------------
 // Utilities 
 //-----------------------------------------------------------------------------
+predicate pageIsFree(d:PageDb, pg:PageNr)
+{
+    wellFormedPageDb(d) && d[pg].PageDbEntryFree?
+}
+
 predicate validL1PTPage(d:PageDb, p:PageNr)
 {
     validPageDb(d) && d[p].PageDbEntryTyped? && d[p].entry.L1PTable?
@@ -324,10 +327,10 @@ predicate validDispatcherPage(d:PageDb, p:PageNr)
     validPageDb(d) && d[p].PageDbEntryTyped? && d[p].entry.Dispatcher?
 }
 
-// a points to an address space and it is closed
+// TODO: delete this redundant alias
 predicate validAddrspacePage(d: PageDb, a: int)
 {
-    wellFormedPageDb(d) && isAddrspace(d, a)
+    isAddrspace(d, a)
 }
 
 predicate nonStoppedL1(d:PageDb, l1:PageNr)
@@ -370,7 +373,7 @@ predicate validMapping(m:Mapping,d:PageDb,a:PageNr)
     && validPageNr(m.l1index) && 0 <= m.l1index < NR_L1PTES
     && validPageNr(m.l2index) && 0 <= m.l2index < NR_L2PTES
     && (var addrspace := d[a].entry;
-        addrspace.state == InitState &&
+        addrspace.state != StoppedState &&
         (var l1 := d[addrspace.l1ptnr].entry;
         l1.l1pt[m.l1index].Just?))
 }
