verified/smcapi.s.dfy
@@ -1,79 +1,7 @@
 include "kom_common.s.dfy"
-include "pagedb.s.dfy"
+include "mapping.s.dfy"
 include "entry.s.dfy"
 include "addrseq.dfy"
-
-predicate pageIsFree(d:PageDb, pg:PageNr)
-{
-    pg in d && d[pg].PageDbEntryFree?
-}
-
-predicate l1indexInUse(d: PageDb, a: PageNr, l1index: int)
-    requires validPageDb(d)
-    requires isAddrspace(d, a)
-    requires !stoppedAddrspace(d[a])
-    requires 0 <= l1index < NR_L1PTES
-{
-    reveal validPageDb();
-    assert validAddrspace(d, a);
-    var l1ptnr := d[a].entry.l1ptnr;
-    var l1pt := d[l1ptnr].entry;
-    l1pt.l1pt[l1index].Just?
-}
-
-function updateL2Pte(d: PageDb, a: PageNr, mapping: Mapping, l2e : L2PTE)
-    : PageDb 
-    requires validPageDb(d)
-    requires isAddrspace(d, a)
-    requires validMapping(mapping,d,a)
-    //requires isValidMappingTarget(d, a, mapping) == KOM_ERR_SUCCESS
-    requires d[a].entry.state.InitState?
-    requires validL2PTE(d, a, l2e)
-    ensures wellFormedPageDb(updateL2Pte(d, a, mapping, l2e))
-{
-    reveal validPageDb();
-    var addrspace := d[a].entry;
-    assert validAddrspace(d, a);
-    var l1 := d[addrspace.l1ptnr].entry;
-    var l1pte := fromJust(l1.l1pt[mapping.l1index]);
-    var l2pt := d[l1pte].entry.l2pt;
-    d[ l1pte := d[l1pte].( entry := d[l1pte].entry.( l2pt := 
-        l2pt[mapping.l2index := l2e] ))]
-}
-
-function isValidMappingTarget(d: PageDb, a: PageNr, mapping: word)
-    : int // KOM_ERROR
-    requires validPageDb(d)
-    requires isAddrspace(d, a)
-    ensures  isValidMappingTarget(d,a,mapping) == KOM_ERR_SUCCESS ==>
-        validMapping(wordToMapping(mapping),d,a)
-{
-    reveal validPageDb();
-    reveal wordToMapping();
-    var addrspace := d[a].entry;
-    var l1index := l1indexFromMapping(mapping);
-    var l2index := l2indexFromMapping(mapping);
-    var perm := permFromMapping(mapping);
-    if(!addrspace.state.InitState?) then
-        KOM_ERR_ALREADY_FINAL
-    else if(!validPageNr(l1indexFromMapping(mapping)) ||
-        !validPageNr(l2indexFromMapping(mapping))) then
-        KOM_ERR_INVALID_MAPPING
-    else 
-        if(!perm.r) then KOM_ERR_INVALID_MAPPING
-        else if(!(0 <= l1index < NR_L1PTES)
-            || !(0 <= l2index < NR_L2PTES) ) then
-            KOM_ERR_INVALID_MAPPING
-        else
-            assert validAddrspace(d, a);
-            var l1 := d[addrspace.l1ptnr].entry;
-            var l1pte := l1.l1pt[l1index];
-            if(l1pte.Nothing?) then KOM_ERR_INVALID_MAPPING
-            else
-                var l2pt := d[fromJust(l1pte)].entry.l2pt;
-                if(!l2pt[l2index].NoMapping?) then KOM_ERR_INVALID_MAPPING
-                else KOM_ERR_SUCCESS
-}
 
 //============================================================================
 // Behavioral Specification of Monitor Calls
@@ -183,27 +111,6 @@ function smc_initDispatcher(pageDbIn: PageDb, page:word, addrspacePage:word,
             (pagedb', err)
 }
 
-function installL1PTE(l1pt: PageDbEntryTyped, l2page: PageNr, l1index: int): PageDbEntryTyped
-    requires l1pt.L1PTable? && wellFormedPageDbEntryTyped(l1pt)
-    requires 0 <= l1index < NR_L1PTES
-    ensures var r := installL1PTE(l1pt, l2page, l1index);
-        r.L1PTable? && wellFormedPageDbEntryTyped(r)
-{
-    l1pt.(l1pt := l1pt.l1pt[l1index := Just(l2page)])
-}
-
-function installL1PTEInPageDb(pagedb: PageDb, l1ptnr: PageNr, l2page: PageNr,
-    l1index: int): PageDb
-    requires validPageDb(pagedb)
-    requires pagedb[l1ptnr].PageDbEntryTyped? && pagedb[l1ptnr].entry.L1PTable?
-    requires 0 <= l1index < NR_L1PTES
-    ensures wellFormedPageDb(installL1PTEInPageDb(pagedb, l1ptnr, l2page, l1index))
-{
-    reveal validPageDb();
-    var l1ptentry := installL1PTE(pagedb[l1ptnr].entry, l2page, l1index);
-    pagedb[l1ptnr := pagedb[l1ptnr].(entry := l1ptentry)]
-}
-
 function smc_initL2PTable(pageDbIn: PageDb, page: word, addrspacePage: word,
                           l1index: word) : (PageDb, word)
     requires validPageDb(pageDbIn)
@@ -298,10 +205,12 @@ function smc_remove(pageDbIn: PageDb, page: word)
         var addrspacePage := pageDbIn[page].addrspace;
         var addrspace := pageDbIn[addrspacePage].entry;
         if( e.Addrspace? ) then
-           if(e.refcount !=0) then (pageDbIn, KOM_ERR_PAGEINUSE)
-           else (pageDbIn[page := PageDbEntryFree], KOM_ERR_SUCCESS)
+            if(e.refcount !=0) then (pageDbIn, KOM_ERR_PAGEINUSE)
+            else (pageDbIn[page := PageDbEntryFree], KOM_ERR_SUCCESS)
         else
-            if( !(addrspace.state.StoppedState? || e.SparePage?) ) then
+            if !addrspace.state.StoppedState?
+                || (e.SparePage? && !addrspace.state.FinalState?) then
+                // TODO: misleading error message for remove of a spare page
                 (pageDbIn, KOM_ERR_NOT_STOPPED)
             else 
                 var d := pageDbIn; var p := page; var a := addrspacePage;
@@ -360,7 +269,7 @@ function smc_mapInsecure(pageDbIn: PageDb, addrspacePage: word,
     reveal validPageDb();
     if(!isAddrspace(pageDbIn, addrspacePage)) then
         (pageDbIn, KOM_ERR_INVALID_ADDRSPACE)
-    else
+    else 
         var err := isValidMappingTarget(pageDbIn, addrspacePage, mapping);
         if( err != KOM_ERR_SUCCESS ) then (pageDbIn, err)
         else if(!physPageIsInsecureRam(physPage)) then
@@ -450,7 +359,7 @@ predicate smchandlerRelation(s: state, pageDbIn: PageDb, s':state, pageDbOut: Pa
         var pg := maybeContentsOfPhysPage(s, arg4);
         (pageDbOut, err) == smc_mapSecure(pageDbIn, arg1, arg2, arg3, arg4, pg) && val == 0
     else if callno == KOM_SMC_ALLOC_SPARE then
-        (pageDbOut, err) == smc_allocSspare(pageDbIn, arg1, arg2) && val == 0
+        (pageDbOut, err) == smc_allocSpare(pageDbIn, arg1, arg2) && val == 0
     else if callno == KOM_SMC_MAP_INSECURE then
         (pageDbOut, err) == smc_mapInsecure(pageDbIn, arg1, arg2, arg3) && val == 0
     else if callno == KOM_SMC_REMOVE then
