verified/mapping.s.dfy
@@ -1,0 +1,99 @@
+include "kom_common.s.dfy"
+include "pagedb.s.dfy"
+
+predicate l1indexInUse(d: PageDb, a: PageNr, l1index: int)
+    requires validPageDb(d)
+    requires isAddrspace(d, a)
+    requires !stoppedAddrspace(d[a])
+    requires 0 <= l1index < NR_L1PTES
+{
+    assert validAddrspace(d, a) by { reveal_validPageDb(); }
+    var l1ptnr := d[a].entry.l1ptnr;
+    var l1pt := d[l1ptnr].entry;
+    l1pt.l1pt[l1index].Just?
+}
+
+function updateL2Pte(d: PageDb, a: PageNr, mapping: Mapping, l2e : L2PTE)
+    : PageDb 
+    requires validPageDb(d)
+    requires isAddrspace(d, a)
+    requires validMapping(mapping,d,a)
+    //requires isValidMappingTarget(d, a, mapping) == KOM_ERR_SUCCESS
+    //requires d[a].entry.state.InitState?
+    requires validL2PTE(d, a, l2e)
+    ensures wellFormedPageDb(updateL2Pte(d, a, mapping, l2e))
+{
+    var addrspace := d[a].entry;
+    assert validAddrspace(d, a) by { reveal_validPageDb(); }
+    var l1 := d[addrspace.l1ptnr].entry;
+    var l1pte := fromJust(l1.l1pt[mapping.l1index]);
+    var l2pt := d[l1pte].entry.l2pt;
+    d[ l1pte := d[l1pte].( entry := d[l1pte].entry.( l2pt := 
+        l2pt[mapping.l2index := l2e] ))]
+}
+
+function isValidMappingTarget'(d: PageDb, a: PageNr, mapping: word)
+    : int // KOM_ERROR
+    requires validPageDb(d)
+    requires isAddrspace(d, a)
+    ensures  isValidMappingTarget'(d,a,mapping) == KOM_ERR_SUCCESS ==>
+        validMapping(wordToMapping(mapping),d,a)
+{
+    reveal validPageDb();
+    reveal wordToMapping();
+    var addrspace := d[a].entry;
+    var l1index := l1indexFromMapping(mapping);
+    var l2index := l2indexFromMapping(mapping);
+    var perm := permFromMapping(mapping);
+    if addrspace.state.StoppedState? then
+        KOM_ERR_STOPPED
+    else if !validPageNr(l1indexFromMapping(mapping)) ||
+        !validPageNr(l2indexFromMapping(mapping)) then
+        KOM_ERR_INVALID_MAPPING
+    else 
+        if(!perm.r) then KOM_ERR_INVALID_MAPPING
+        else if(!(0 <= l1index < NR_L1PTES)
+            || !(0 <= l2index < NR_L2PTES) ) then
+            KOM_ERR_INVALID_MAPPING
+        else
+            assert validAddrspace(d, a);
+            var l1 := d[addrspace.l1ptnr].entry;
+            var l1pte := l1.l1pt[l1index];
+            if(l1pte.Nothing?) then KOM_ERR_INVALID_MAPPING
+            else
+                var l2pt := d[fromJust(l1pte)].entry.l2pt;
+                if(!l2pt[l2index].NoMapping?) then KOM_ERR_INVALID_MAPPING
+                else KOM_ERR_SUCCESS
+}
+
+function isValidMappingTarget(d: PageDb, a: PageNr, mapping: word)
+    : int // KOM_ERROR
+    requires validPageDb(d)
+    requires isAddrspace(d, a)
+    ensures  isValidMappingTarget(d,a,mapping) == KOM_ERR_SUCCESS ==>
+        validMapping(wordToMapping(mapping),d,a)
+{
+    if !d[a].entry.state.InitState? then KOM_ERR_ALREADY_FINAL
+    else isValidMappingTarget'(d, a, mapping)
+}
+
+function installL1PTE(l1pt: PageDbEntryTyped, l2page: PageNr, l1index: int): PageDbEntryTyped
+    requires l1pt.L1PTable? && wellFormedPageDbEntryTyped(l1pt)
+    requires 0 <= l1index < NR_L1PTES
+    ensures var r := installL1PTE(l1pt, l2page, l1index);
+        r.L1PTable? && wellFormedPageDbEntryTyped(r)
+{
+    l1pt.(l1pt := l1pt.l1pt[l1index := Just(l2page)])
+}
+
+function installL1PTEInPageDb(pagedb: PageDb, l1ptnr: PageNr, l2page: PageNr,
+    l1index: int): PageDb
+    requires wellFormedPageDb(pagedb)
+    requires pagedb[l1ptnr].PageDbEntryTyped? && pagedb[l1ptnr].entry.L1PTable?
+    requires 0 <= l1index < NR_L1PTES
+    ensures wellFormedPageDb(installL1PTEInPageDb(pagedb, l1ptnr, l2page, l1index))
+{
+    //reveal validPageDb();
+    var l1ptentry := installL1PTE(pagedb[l1ptnr].entry, l2page, l1index);
+    pagedb[l1ptnr := pagedb[l1ptnr].(entry := l1ptentry)]
+}
