verified/smcapi.i.dfy
@@ -263,35 +263,6 @@ lemma initDispatcherPreservesPageDBValidity(pageDbIn:PageDb, page:word, addrspac
     }
 }
 
-lemma installL1PTEPreservesPageDbValidity(pageDbIn: PageDb, l1ptnr: PageNr,
-                                          l2page: PageNr, l1index: int)
-    requires validPageDb(pageDbIn)
-    requires pageDbIn[l1ptnr].PageDbEntryTyped? && pageDbIn[l1ptnr].entry.L1PTable?
-    // l2page belongs to this addrspace
-    requires validL1PTE(pageDbIn, l2page)
-        && pageDbIn[l2page].addrspace == pageDbIn[l1ptnr].addrspace
-    // no double mapping
-    requires forall i :: 0 <= i < NR_L1PTES && i != l1index
-        ==> pageDbIn[l1ptnr].entry.l1pt[i] != Just(l2page)
-    requires 0 <= l1index < NR_L1PTES
-    ensures validPageDb(installL1PTEInPageDb(pageDbIn, l1ptnr, l2page, l1index))
-{
-    reveal validPageDb();
-
-    assert validL1PTable(pageDbIn, l1ptnr);
-    var pageDbOut := installL1PTEInPageDb(pageDbIn, l1ptnr, l2page, l1index);
-
-    assert validL1PTable(pageDbOut, l1ptnr);
-
-    forall ( n | validPageNr(n) && n != l1ptnr)
-        ensures validPageDbEntry(pageDbOut, n)
-    {
-        assert pageDbOut[n] == pageDbIn[n];
-        assert validPageDbEntry(pageDbIn, n);
-        assert addrspaceRefs(pageDbOut, n) == addrspaceRefs(pageDbIn, n);
-    }
-}
-
 lemma initL2PTablePreservesPageDBValidity(pageDbIn: PageDb, page: word,
     addrspacePage: word, l1index: word)
     requires validPageDb(pageDbIn)
@@ -341,16 +312,13 @@ lemma removePreservesPageDBValidity(pageDbIn: PageDb, page: word)
         var addrspacePage := pageDbIn[page].addrspace;
         assert validAddrspace(pageDbIn, addrspacePage);
 
-        forall () ensures validPageDbEntry(pageDbOut, addrspacePage);
-        {
-            if(entry.Addrspace?){
-            } else {
+        assert validPageDbEntry(pageDbOut, addrspacePage) by {
+            if !entry.Addrspace? {
                 var addrspace := pageDbOut[addrspacePage].entry;
 
                 var oldRefs := addrspaceRefs(pageDbIn, addrspacePage);
                 assert addrspaceRefs(pageDbOut, addrspacePage) == oldRefs - {page};
                 assert addrspace.refcount == |addrspaceRefs(pageDbOut, addrspacePage)|;
-                
                 //assert validAddrspace(pageDbOut, addrspace);
                 assert validAddrspacePage(pageDbOut, addrspacePage);
             }
@@ -723,86 +691,6 @@ lemma smchandlerPreservesPageDbValidity(s: state, pageDbIn: PageDb, s':state,
     } else if(callno == KOM_SMC_STOP) {
         stopPreservesPageDbValidity(pageDbIn, arg1);
     }
-}
-
-lemma lemma_updateL2PtePreservesPageDb(d:PageDb,a:PageNr,mapping:Mapping,l2e:L2PTE) 
-    requires validPageDb(d)
-    requires isAddrspace(d, a)
-    requires validMapping(mapping,d,a)
-    requires d[a].entry.state.InitState?
-    requires validL2PTE(d,a,l2e)
-    ensures validPageDb(updateL2Pte(d,a,mapping,l2e))
-{
-    reveal validPageDb();
-    var d' := updateL2Pte(d,a,mapping,l2e);
-    
-    var addrspace := d[a].entry;
-    assert validAddrspace(d, a);
-
-    var l2index := mapping.l2index;
-    var l1index := mapping.l1index;
-
-    var l1p := d[a].entry.l1ptnr;
-    var l1 := d[l1p].entry;
-    var l1p' := d'[a].entry.l1ptnr;
-    var l1' := d'[l1p'].entry;
-    assert l1p' == l1p;
-    assert l1' == l1;
-
-    var l1pte := fromJust(l1.l1pt[l1index]);
-    var l1pte' := fromJust(l1'.l1pt[l1index]);
-    assert l1pte == l1pte';
-    var l2pt := d[l1pte].entry.l2pt;
-    var l2pt' := d'[l1pte].entry.l2pt;
-
-    //it's now okay to drop the primes from everything but l2pt'
-
-    assert !stoppedAddrspace(d[a]);
-    assert !stoppedAddrspace(d'[a]);
-
-    assert validPageDbEntry(d, a);
-    assert validPageDbEntry(d', a) by
-    {
-        assert d'[a].entry.refcount == d[a].entry.refcount;
-        assert addrspaceRefs(d', a) == addrspaceRefs(d, a);
-        
-    }
-
-    assert validPageDbEntry(d, l1p);
-    assert validPageDbEntry(d, l1pte);
-
-    assert validPageDbEntry(d', l1p);
-    assert validPageDbEntry(d', l1pte) by
-    {
-       assert d'[l1pte].entry.L2PTable?;
-       assert !stoppedAddrspace(d'[a]);
-       assert validL2PTE(d',a,l2e);
-       assert wellFormedPageDbEntryTyped(d[l1pte].entry);
-       assert wellFormedPageDbEntryTyped(d'[l1pte].entry);
-
-       assert |l2pt| == |l2pt'|;
-
-       forall ( i | 0 <= i < NR_L2PTES && i != l2index )
-            ensures validL2PTE(d',a,l2pt'[i])
-       {
-            assert l2pt'[i] == l2pt[i];
-            assert validL2PTE(d,a,l2pt[i]);
-       }
-
-    }
-
-    forall ( p | validPageNr(p) && p != l1p && p != l1pte && p != a )
-        ensures validPageDbEntry(d', p)
-    {
-            assert d'[p] == d[p];
-            assert validPageDbEntry(d, p);
-            assert addrspaceRefs(d', p) == addrspaceRefs(d, p);
-    }
-    
-    assert wellFormedPageDb(d');
-    assert pageDbEntriesValid(d');
-    assert pageDbEntriesValidRefs(d');
-  
 }
 
 lemma kom_smc_map_measure_helper1(s:state, as_page:PageNr, metadata:seq<word>, contents:seq<word>, pagedb_in:PageDb)
