verified/svcapi.i.dfy
@@ -1,0 +1,84 @@
+include "svcapi.s.dfy"
+include "pagedb.i.dfy"
+include "mapping.i.dfy"
+
+lemma lemma_svcMapData_validPageDb(d:PageDb, asPg:PageNr, page:word, mapping:word)
+    requires validPageDb(d) && validAddrspacePage(d, asPg)
+    ensures validPageDb(svcMapData(d, asPg, page, mapping).0)
+{
+    var rd := svcMapData(d, asPg, page, mapping).0;
+    if rd != d {
+        var datapg := DataPage(SeqRepeat(PAGESIZE/WORDSIZE, 0));
+        var abs_mapping := wordToMapping(mapping);
+        var l2pte := SecureMapping(page, abs_mapping.perm.w, abs_mapping.perm.x);
+        lemma_allocateSparePage(d, page, datapg);
+        lemma_updateL2PtePreservesPageDb(allocateSparePage(d, page, datapg),
+            asPg, abs_mapping, l2pte);
+    }
+}
+
+lemma lemma_svcInitL2PTable_validPageDb(d:PageDb, asPg:PageNr, page:word, l1index:word)
+    requires validPageDb(d) && validAddrspacePage(d, asPg) && d[asPg].entry.state.FinalState?
+    ensures validPageDb(svcInitL2PTable(d, asPg, page, l1index).0)
+{
+    reveal validPageDb();
+    
+    var rd := svcInitL2PTable(d, asPg, page, l1index).0;
+    if rd != d {
+        var l1ptnr := d[asPg].entry.l1ptnr;
+        var l1pt := d[l1ptnr].entry.l1pt;
+
+        // no refs to the free page
+        forall (i | 0 <= i < NR_L1PTES)
+            ensures l1pt[i] != Just(page)
+        {
+            assert validSparePageForAS(d, asPg, page);
+            assert !stoppedAddrspace(d[asPg]);
+            assert validL1PTable(d, l1ptnr);
+            assert l1pt[i].Just? ==> validL1PTE(d, fromJust(l1pt[i]));
+        }
+
+        var l2pt := L2PTable(SeqRepeat(NR_L2PTES, NoMapping));
+        var d1 := allocateSparePage(d, page, l2pt);
+        lemma_allocateSparePage(d, page, l2pt);
+        var d2 := installL1PTEInPageDb(d1, l1ptnr, page, l1index);
+        installL1PTEPreservesPageDbValidity(d1, l1ptnr, page, l1index);
+    }
+}
+
+lemma lemma_svcHandled_validPageDb(s:state, sd:PageDb, dispPg:PageNr, regs:SvcReturnRegs, rd:PageDb)
+    requires ValidState(s) && mode_of_state(s) != User
+    requires validPageDb(sd) && validDispatcherPage(sd, dispPg)
+    requires isReturningSvc(s)
+    requires finalDispatcher(sd, dispPg)
+    requires validPageNr(l1pOfDispatcher(sd, dispPg))
+    requires (regs, rd) == svcHandled(s, sd, dispPg)
+    ensures validPageDb(rd)
+{
+    reveal validPageDb();
+    var addrspace := sd[dispPg].addrspace;
+    assert validAddrspacePage(sd, addrspace);
+
+    if regs.0 != KOM_ERR_SUCCESS {
+        assert rd == sd;
+    } else if s.regs[R0] == KOM_SVC_ATTEST || s.regs[R0] == KOM_SVC_VERIFY_STEP2 {
+        assert rd == sd;
+    } else if s.regs[R0] == KOM_SVC_VERIFY_STEP0 || s.regs[R0] == KOM_SVC_VERIFY_STEP1 {
+        forall n | validPageNr(n) ensures validPageDbEntry(rd, n)
+        {
+            var e := rd[n];
+            if (e.PageDbEntryTyped?)
+            {
+                var entry := e.entry;
+                if (entry.Addrspace?)
+                {
+                    assert addrspaceRefs(rd, n) == addrspaceRefs(sd, n); // set equality
+                }
+            }
+        }
+    } else if s.regs[R0] == KOM_SVC_MAP_DATA {
+        lemma_svcMapData_validPageDb(sd, addrspace, s.regs[R1], s.regs[R2]);
+    } else if s.regs[R0] == KOM_SVC_INIT_L2PTABLE {
+        lemma_svcInitL2PTable_validPageDb(sd, addrspace, s.regs[R1], s.regs[R2]);
+    }
+}
